update

coq.v
@@ -2,88 +2,17 @@ Require Import Bool Arith List.
 Set Implicit Arguments.
 Set Asymmetric Patterns.
 
-Inductive binop : Set := Plus | Times.
-Inductive exp: Set :=
-|Const : nat -> exp
-|Binop : binop -> exp -> exp -> exp.
-
-Inductive instr : Set :=
-| iConst : nat -> instr
-| iBinop : binop -> instr.
-
-Definition prog := list instr.
-Definition stack := list nat.
-
-Definition binopDenote ( b: binop) : nat -> nat -> nat :=
-    match b with
-    | Plus => plus
-    | Times => mult
+Definition nandb (b1 b2 :bool) : bool :=
+    match b1 with
+    | true => negb b2
+    | false => true
     end.
-
-Fixpoint expDenote (e:exp) : nat :=
-    match e with
-    | Const n => n
-    | Binop b e1 e2 => (binopDenote b) (expDenote e1) (expDenote e2)
-    end.
-
-Definition instrDenote (i:instr) (s:stack) : option stack :=
-    match i with
-    | iConst n => Some (n::s)
-    | iBinop b => 
-        match s with
-        | arg1 :: arg2 :: s' => Some ((binopDenote b) arg1 arg2 :: s')
-        | _ => None
-        end
-    end.
-Fixpoint progDenote (p:prog) (s:stack) : option stack :=
-    match p with
-    | nil => Some s
-    | i :: p' =>
-        match instrDenote i s with
-        | None => None
-        | Some s' => progDenote p' s'
-        end
-    end.
-Fixpoint compile (e:exp) : prog :=
-    match e with
-    |Const n => iConst n :: nil
-    | Binop b e1 e2 => compile e2 ++ compile e1 ++ iBinop b::nil
-    end.
-Lemma compile_correct' : forall e p s, progDenote (compile e ++ p) s = progDenote p ( expDenote e::s).
+Example test_nandb1: (nandb true false) = true.
 Proof.
-    induction e.
-    intros.
-    unfold compile.
-    unfold expDenote.
-    unfold progDenote at 1.
-    simpl.
-    fold progDenote.
-    reflexivity.
-    intros.
-    simpl.
-    rewrite <- app_assoc.
-    rewrite IHe2.
-    rewrite <- app_assoc.
-    rewrite IHe1.
     simpl.
     reflexivity.
     Qed.
-Theorem compile_correct : forall e, progDenote (compile e) nil = Some (expDenote e::nil).
-Proof.
-    intros.
-    rewrite <- (app_nil_r (compile e)).
-    rewrite compile_correct'.
-    simpl.
-    reflexivity.
-    Qed.
-    
-Theorem compile_correct2 : forall e, progDenote (compile e) nil = Some (expDenote e::nil).
-Proof.
-    intros.
-    rewrite <- (app_nil_r (compile e)).
-    induction e.
-    simpl.
-    reflexivity.
-    simpl.
-    rewrite <- app_assoc.
-    rewrite IHe2.
+
+Check negb.
+
+Inductive rgb :
